wip

src/drf/AbortProp.v
@@ -126,25 +126,22 @@ Inductive concreter_memory (mem_src mem_tgt: Memory.t): Prop :=
         Memory.get loc to mem_src = Some (from, Message.full val vw))
 .
 
-Lemma concreter_memory_write mem_src0 mem_tgt0 prom0
-      loc from to val vw_src vw_tgt prom1 mem_tgt1 kind
-      (CONCRETE: concreter_memory mem_src0 mem_tgt0)
-      (MLESRC: Memory.le prom0 mem_src0)
-      (MLETGT: Memory.le prom0 mem_tgt0)
-      (VWLE: View.opt_le vw_src vw_tgt)
-      (VWWF: View.opt_wf vw_src)
-      (WRITE: Memory.write prom0 mem_tgt0 loc from to val vw_tgt prom1 mem_tgt1 kind)
-  :
-    exists mem_src1,
-      (<<PROMISE: Memory.write prom0 mem_src0 loc from to val vw_src prom1 mem_src1 kind>>) /\
-      (<<CONCRETE: concreter_memory mem_src1 mem_tgt1>>).
-Proof.
-  inv WRITE. inv PROMISE.
-  -
-
-
-
-Lemma concret
+(* Lemma concreter_memory_write mem_src0 mem_tgt0 prom0 *)
+(*       loc from to val vw_src vw_tgt prom1 mem_tgt1 kind *)
+(*       (CONCRETE: concreter_memory mem_src0 mem_tgt0) *)
+(*       (MLESRC: Memory.le prom0 mem_src0) *)
+(*       (MLETGT: Memory.le prom0 mem_tgt0) *)
+(*       (VWLE: View.opt_le vw_src vw_tgt) *)
+(*       (VWWF: View.opt_wf vw_src) *)
+(*       (WRITE: Memory.write prom0 mem_tgt0 loc from to val vw_tgt prom1 mem_tgt1 kind) *)
+(*   : *)
+(*     exists mem_src1, *)
+(*       (<<PROMISE: Memory.write prom0 mem_src0 loc from to val vw_src prom1 mem_src1 kind>>) /\ *)
+(*       (<<CONCRETE: concreter_memory mem_src1 mem_tgt1>>). *)
+(* Proof. *)
+(*   inv WRITE. inv PROMISE. *)
+(*   - exploit add_succeed_wf; try apply PROMISES. i. des. *)
+(*     exploit add_succeed_wf; try apply MEM. i. des. *)
 
 Lemma concreter_memory_step
       lang prom th_src th_tgt th_tgt' st st' vw vw' prom' sc sc'
@@ -165,8 +162,141 @@ Lemma concreter_memory_step
       (<<CONCRETE: concreter_memory mem_src' mem_tgt'>>)
 .
 Proof.
+Admitted.
+
+Lemma progressable_in_added_rtc
+      lang st lc sc0 sc1 m0 m1 tm
+      (CONSISTENT: Thread.consistent (Thread.mk lang st lc sc0 m0))
+      (FUTURE: Memory.future m0 m1)
+  :
+    exists m2 e2,
+      (<<ADDED: rtc (added_memory tm) m1 m2>>) /\
+      (<<STEPS: rtc (Thread.tau_step (lang:=lang))
+                    (Thread.mk _ st lc sc1 m1) e2>>) /\
+      (<<PROMISES: Local.promises (Thread.local e2) = Memory.bot>>).
+Proof.
+Admitted.
+
+Lemma promise_free_no_promise P lang (th0 th1: Thread.t lang) e
+      (NOPROMISE: th0.(Thread.local).(Local.promises) = Memory.bot)
+      (STEP: pred_step (P /1\ promise_free) e th0 th1)
+  :
+    (<<STEP: pred_step (P /1\ no_promise) e th0 th1>>) /\
+    (<<NOPROMISE: th1.(Thread.local).(Local.promises) = Memory.bot>>).
+Proof.
+  inv STEP. inv STEP0. inv STEP.
+  - inv STEP0. inv LOCAL. inv PROMISE; ss; des; clarify.
+    + rewrite NOPROMISE in *.
+      eapply Memory.lower_get0 in PROMISES. des.
+      erewrite Memory.bot_get in *. clarify.
+    + rewrite NOPROMISE in *.
+      eapply Memory.remove_get0 in PROMISES. des.
+      erewrite Memory.bot_get in *. clarify.
+  - inv STEP0. inv LOCAL.
+    + ss. esplits; eauto. econs; eauto. econs; eauto.
+    + ss. esplits; eauto.
+      * econs; eauto. econs; eauto.
+      * inv LOCAL0. ss.
+    + ss. esplits; eauto.
+      * econs; eauto. econs; eauto.
+      * inv LOCAL0. rewrite NOPROMISE in *.
+        exploit memory_write_bot_add; eauto. i. clarify.
+        inv WRITE. inv PROMISE. ss.
+        symmetry. eapply MemoryMerge.MemoryMerge.add_remove; eauto.
+    + ss. esplits; eauto.
+      * econs; eauto. econs; eauto.
+      * inv LOCAL1. inv LOCAL2. rewrite NOPROMISE in *.
+        exploit memory_write_bot_add; eauto. i. clarify.
+        inv WRITE. inv PROMISE. ss.
+        symmetry. eapply MemoryMerge.MemoryMerge.add_remove; eauto.
+    + ss. esplits; eauto.
+      * econs; eauto. econs; eauto.
+      * inv LOCAL0. ss.
+    + ss. esplits; eauto.
+      * econs; eauto. econs; eauto.
+      * inv LOCAL0. ss.
+    + ss. esplits; eauto.
+      * econs; eauto. econs; eauto.
+Qed.
+
+Definition pf_consistent_strong lang (e:Thread.t lang): Prop :=
+  forall mem1 sc1
+         (WF: Local.wf e.(Thread.local) e.(Thread.memory))
+         (MEM: Memory.closed e.(Thread.memory))
+         (CAP: Memory.cap e.(Thread.local).(Local.promises) e.(Thread.memory) mem1),
+  exists e2 e3,
+    (<<STEPS: rtc (tau (@pred_step (no_sc /1\ promise_free) lang)) (Thread.mk _ e.(Thread.state) e.(Thread.local) sc1 mem1) e2>>) /\
+    (<<FAILURE: pred_step (no_sc /1\ promise_free) (ThreadEvent.failure) e2 e3>>) \/
+    exists e2,
+      (<<STEPS: rtc (tau (@pred_step (no_sc /1\ promise_free) lang)) (Thread.mk _ e.(Thread.state) e.(Thread.local) sc1 mem1) e2>>) /\
+      (<<PROMISES: e2.(Thread.local).(Local.promises) = Memory.bot>>).
+
+Lemma write_promises_decrease prom0 mem0 loc from to val realeased prom1 mem1 kind
+      (WRITE: Memory.write prom0 mem0 loc from to val realeased prom1 mem1 kind)
+  :
+    concrete_promised prom1 <2= concrete_promised prom0.
+Proof.
+  inv WRITE. inv PROMISE.
+  - exploit MemoryMerge.MemoryMerge.add_remove.
+    + eapply PROMISES.
+    + eapply REMOVE.
+    + i. clarify.
+  - ii. inv PR.
+    erewrite Memory.remove_o in GET; eauto. des_ifs.
+    erewrite Memory.split_o in GET; eauto. des_ifs.
+    + ss; des; clarify.
+    + ss. des; clarify. eapply Memory.split_get0 in PROMISES.
+      des. econs; eauto.
+    + eapply Memory.split_get0 in PROMISES.
+      guardH o. guardH o0. guardH o1. des. econs; eauto.
+  - ii. inv PR.
+    erewrite Memory.remove_o in GET; eauto. des_ifs.
+    erewrite Memory.lower_o in GET; eauto. des_ifs.
+    + ss; des; clarify.
+    + econs; eauto.
+  - clarify.
+Qed.
+
+Lemma pf_step_promises_decrease
 
 
+
+
+
+Lemma pf_consistent_pf_consistent_strong lang (th: Thread.t lang)
+      (CONSISTENT: pf_consistent th)
+  :
+    pf_consistent_strong th.
+Proof.
+  ii.
+
+  exploit Memory.cap_exists
+
+  inv CONSISTENT.
+
+Local.wf (Thread.local e) (Thread.memory e) ->
+Memory.closed (Thread.memory e) ->
+Memory.cap (Local.promises (Thread.local e)) (Thread.memory e) mem1 ->
+Memory.max_full_timemap mem1 sc1 ->
+
+
+
+Local.p
+
+
+.
+
+
+
+
+    (<<FAILURE: Thread.steps_failure (Thread.mk _ e.(Thread.state) e.(Thread.local) sc1 mem1)>>) \/
+    exists e2,
+      (<<STEPS: rtc (tau (Thread.step true)) (Thread.mk _ e.(Thread.state) e.(Thread.local) sc1 mem1) e2>>) /\
+      (<<PROMISES: e2.(Thread.local).(Local.promises) = Memory.bot>>).
+
+
+
+Memory.finite
 
 
 Lemma concreter_memory_promise mem_src0 mem_tgt0 prom0
@@ -218,381 +348,3 @@ Lemma concreter_memory_promise mem_src0 mem_tgt0 prom0
 Proof.
   inv WRITE. inv PROMISE.
   -
-
-
-
-Admitted.
-
-
-
-
-
-
-        exists from_src vw_src,
-          (<<GETSRC: Memory.get loc to mem_src = Some (from_src, Message.full val vw_src)>>) /\
-          (<<VWLE: View.opt_le vw_src vw_tgt>>)).
-
-
-    ()
-
-
-
-
-Inductive lower_memory (mem_src mem_tgt: Memory.t): Prop :=
-| lower_memory_intro
-    (COVER: forall loc to (COV: covered loc to mem_src),
-        covered loc to mem_tgt)
-    (MLE: forall loc to from_tgt vw_tgt val
-                 (GETTGT: Memory.get loc to mem_tgt = Some (from_tgt, Message.full val vw_tgt)),
-        exists from_src vw_src,
-          (<<GETSRC: Memory.get loc to mem_src = Some (from_src, Message.full val vw_src)>>) /\
-          (<<VWLE: View.opt_le vw_src vw_tgt>>)).
-
-Definition pf_consistent_strong lang (e:Thread.t lang): Prop :=
-  forall mem1 sc1
-         (WF: Local.wf e.(Thread.local) e.(Thread.memory))
-         (MEM: Memory.closed e.(Thread.memory))
-         (CAP: Memory.cap e.(Thread.local).(Local.promises) e.(Thread.memory) mem1),
-    (<<FAILURE: Thread.steps_failure (Thread.mk _ e.(Thread.state) e.(Thread.local) sc1 mem1)>>) \/
-    exists e2,
-      (<<STEPS: rtc (tau (Thread.step true)) (Thread.mk _ e.(Thread.state) e.(Thread.local) sc1 mem1) e2>>) /\
-      (<<PROMISES: e2.(Thread.local).(Local.promises) = Memory.bot>>).
-
-
-
-Inductive lower_event: ThreadEvent.t -> ThreadEvent.t -> Prop :=
-| lower_event_silent:
-    lower_event ThreadEvent.silent ThreadEvent.silent
-| lower_event_syscall e:
-    lower_event (ThreadEvent.syscall e) (ThreadEvent.syscall e)
-| lower_event_failure:
-    lower_event ThreadEvent.failure ThreadEvent.failure
-| lower_event_fence ordr ordw:
-    lower_event (ThreadEvent.fence ordr ordw) (ThreadEvent.fence ordr ordw)
-| lower_event_read
-    loc to val vw_src vw_tgt ordr
-    (VWLE: View.opt_le vw_src vw_tgt)
-  :
-    lower_event
-      (ThreadEvent.read loc to val vw_src ordr)
-      (ThreadEvent.read loc to val vw_tgt ordr)
-| lower_event_write
-    loc from to val vw_src vw_tgt ordw
-    (VWLE: View.opt_le vw_src vw_tgt)
-  :
-    lower_event
-      (ThreadEvent.write loc from to val vw_src ordw)
-      (ThreadEvent.write loc from to val vw_tgt ordw)
-| lower_event_update
-    loc from to valr valw vwr_src vwr_tgt vww_src vww_tgt ordr ordw
-    (VWRLE: View.opt_le vwr_src vwr_tgt)
-    (VWWLE: View.opt_le vww_src vww_tgt)
-  :
-    lower_event
-      (ThreadEvent.update loc from to valr valw vwr_src vww_src ordr ordw)
-      (ThreadEvent.update loc from to valr valw vwr_tgt vww_tgt ordr ordw)
-| lower_event_promise
-    loc from to msg kind
-  :
-    lower_event
-      (ThreadEvent.promise loc from to msg kind)
-      (ThreadEvent.promise loc from to msg kind)
-.
-Hint Constructors lower_event.
-
-Lemma lower_memory_closed_message msg mem_src mem_tgt
-      (LOWMEM: lower_memory mem_src mem_tgt)
-      (CLOSED: Memory.closed_message msg mem_tgt)
-  :
-    Memory.closed_message msg mem_src.
-Proof.
-  inv CLOSED; eauto. inv CLOSED0; eauto. econs. econs.
-  inv CLOSED. inv LOWMEM. econs.
-  - ii. specialize (PLN loc). des.
-    eapply MLE in PLN. des. esplits; eauto.
-  - ii. specialize (RLX loc). des.
-    eapply MLE in RLX. des. esplits; eauto.
-Qed.
-
-Lemma promise_consistent_mon v_src v_tgt prom
-      (CONSISTENT: Local.promise_consistent (Local.mk v_tgt prom))
-      (VWLE: TView.le v_src v_tgt)
-  :
-    Local.promise_consistent (Local.mk v_src prom).
-Proof.
-  ii. ss. exploit CONSISTENT; eauto. i. ss.
-  eapply TimeFacts.le_lt_lt; eauto. eapply VWLE.
-Qed.
-
-Lemma lower_memory_promise mem_src0 mem_tgt0 prom0
-      loc from to msg prom1 mem_tgt1 kind
-      (LOWMEM: lower_memory mem_src0 mem_tgt0)
-      (MLESRC: Memory.le prom0 mem_src0)
-      (MLETGT: Memory.le prom0 mem_tgt0)
-      (PROMISE: Memory.promise prom0 mem_tgt0 loc from to msg prom1 mem_tgt1 kind)
-  :
-    exists mem_src1,
-      (<<PROMISE: Memory.promise prom0 mem_src0 loc from to msg prom1 mem_src1 kind>>) /\
-      (<<LOWMEM: lower_memory mem_src1 mem_tgt1>>).
-Proof.
-Admitted.
-
-Lemma lower_memory_write mem_src0 mem_tgt0 prom0
-      loc from to val vw_src vw_tgt prom1 mem_tgt1 kind
-      (LOWMEM: lower_memory mem_src0 mem_tgt0)
-      (MLESRC: Memory.le prom0 mem_src0)
-      (MLETGT: Memory.le prom0 mem_tgt0)
-      (VWLE: View.opt_le vw_src vw_tgt)
-      (VWWF: View.opt_wf vw_src)
-      (PROMISE: Memory.write prom0 mem_tgt0 loc from to val vw_tgt prom1 mem_tgt1 kind)
-  :
-    exists mem_src1,
-      (<<PROMISE: Memory.write prom0 mem_src0 loc from to val vw_src prom1 mem_src1 kind>>) /\
-      (<<LOWMEM: lower_memory mem_src1 mem_tgt1>>).
-Proof.
-Admitted.
-
-Lemma tview_read_fence_wf
-      ord tview
-      (WF_TVIEW: TView.wf tview)
-  :
-    TView.wf (TView.read_fence_tview tview ord).
-Proof.
-  econs; ss; eauto.
-  - i. eapply WF_TVIEW.
-  - des_ifs; eapply WF_TVIEW.
-  - eapply WF_TVIEW.
-  - i. des_ifs; try eapply WF_TVIEW.
-    etrans; eapply WF_TVIEW.
-  - des_ifs; try eapply WF_TVIEW. refl.
-Qed.
-
-Lemma lower_memory_step
-      lang prom th_src th_tgt th_tgt' st st' v_src v_tgt v_tgt' prom' sc_src sc_tgt sc_tgt'
-      mem_src mem_tgt mem_tgt' tf e_tgt
-      (VWFSRC: TView.wf v_src)
-      (VWFTGT: TView.wf v_tgt)
-      (VIEW: TView.le v_src v_tgt)
-      (SC: TimeMap.le sc_src sc_tgt)
-      (TH_SRC: th_src = Thread.mk lang st (Local.mk v_src prom) sc_src mem_src)
-      (TH_TGT0: th_tgt = Thread.mk lang st (Local.mk v_tgt prom) sc_tgt mem_tgt)
-      (TH_TGT1: th_tgt' = Thread.mk lang st' (Local.mk v_tgt' prom') sc_tgt' mem_tgt')
-      (LOWMEM: lower_memory mem_src mem_tgt)
-      (MLESRC: Memory.le prom mem_src)
-      (MLETGT: Memory.le prom mem_tgt)
-      (STEP: Thread.step tf e_tgt th_tgt th_tgt')
-  :
-    exists e_src v_src' mem_src' sc_src',
-      (<<STEP: Thread.step
-                 tf e_src th_src
-                 (Thread.mk lang st' (Local.mk v_src' prom') sc_src' mem_src')>>) /\
-      (<<VIEW: TView.le v_src' v_tgt'>>) /\
-      (<<LOWMEM: lower_memory mem_src' mem_tgt'>>) /\
-      (<<EVT: lower_event e_src e_tgt>>) /\
-      (<<SC: TimeMap.le sc_src' sc_tgt'>>)
-.
-Proof.
-  clarify. inv STEP.
-  - inv STEP0. inv LOCAL. clarify. ss.
-    exploit lower_memory_promise; eauto. i. des. esplits; eauto.
-    econs; eauto. econs 1; eauto. econs; eauto.
-    eapply lower_memory_closed_message; eauto.
-  - inv STEP0. inv LOCAL.
-    + exists ThreadEvent.silent. esplits; eauto.
-    + inv LOCAL0. ss. clarify. dup LOWMEM. inv LOWMEM.
-      exploit MLE; eauto. i. des.
-      exists (ThreadEvent.read loc ts val vw_src ord). esplits; eauto.
-      * econs 2; eauto. econs; eauto. econs; eauto. econs; eauto. ss.
-        eapply TViewFacts.readable_mon; eauto.
-        { inv VIEW. eauto. }
-        { refl. }
-      * ss. eapply TViewFacts.read_tview_mon; eauto.
-        { eapply Cell.get_opt_wf in GET. inv GET. eauto. }
-        { refl. }
-    + inv LOCAL0. ss. clarify.
-      assert (RELEASEDLE:
-                View.opt_le
-                  (TView.write_released v_src sc_src loc to None ord)
-                  (TView.write_released v_tgt sc_tgt loc to None ord)).
-      { eapply TViewFacts.write_released_mon; eauto. refl. }
-      exploit lower_memory_write; eauto.
-      { eapply TViewFacts.write_future0; eauto. } i. des.
-      dup LOWMEM. inv LOWMEM.
-      exists (ThreadEvent.write loc from to val (TView.write_released v_src sc_src loc to None ord) ord).
-      esplits; eauto.
-      * econs 2; eauto. econs; eauto. econs; eauto. econs; eauto. ss.
-        eapply TViewFacts.writable_mon; eauto.
-        { inv VIEW. eauto. }
-        { refl. }
-      * ss. eapply TViewFacts.write_tview_mon; eauto. refl.
-    + inv LOCAL1. inv LOCAL2. ss. clarify.
-      dup LOWMEM. inv LOWMEM.
-      exploit MLE; eauto. i. des.
-      exists (ThreadEvent.update
-                loc tsr tsw valr valw vw_src
-                (TView.write_released (TView.read_tview v_src loc tsr vw_src ordr) sc_src loc tsw
-                                      vw_src ordw) ordr ordw).
-      assert (RELEASEDLE: View.opt_le
-                            (TView.write_released (TView.read_tview v_src loc tsr vw_src ordr) sc_src loc tsw vw_src ordw)
-                            (TView.write_released (TView.read_tview v_tgt loc tsr releasedr ordr) sc_tgt loc tsw
-                                                  releasedr ordw)).
-      { dup GET. eapply Cell.get_opt_wf in GET. inv GET.
-        eapply TViewFacts.write_released_mon; try eassumption.
-        - eapply TViewFacts.read_tview_mon; eauto. refl.
-        - eapply TViewFacts.read_future1; eauto.
-        - refl. }
-      exploit lower_memory_write; try apply WRITE; try eassumption.
-      { dup GETSRC. eapply Cell.get_opt_wf in GETSRC. inv GETSRC.
-        ss. eapply TViewFacts.write_future0; eauto.
-        eapply TViewFacts.read_future1; eauto. }
-      i. des.
-      esplits; eauto.
-      * econs 2; eauto. econs; eauto. econs; eauto.
-        { econs; eauto. ss.
-          eapply TViewFacts.readable_mon; eauto.
-          - eapply VIEW; eauto.
-          - refl. }
-        { econs; eauto. ss.
-          eapply TViewFacts.writable_mon; eauto.
-          - eapply View.join_le.
-            + eapply View.join_le; eauto.
-              * eapply VIEW.
-              * refl.
-            + des_ifs.
-              * eapply View.unwrap_opt_le; eauto.
-              * refl.
-          - refl. }
-      * ss. eapply TViewFacts.write_tview_mon; eauto.
-        { eapply TViewFacts.read_tview_mon; eauto.
-          - dup GET. eapply Cell.get_opt_wf in GET. inv GET. eauto.
-          - refl. }
-        { eapply TViewFacts.read_future1; eauto.
-          dup GET. eapply Cell.get_opt_wf in GET. inv GET. eauto. }
-        { refl. }
-    + inv LOCAL0. ss. clarify. esplits; eauto.
-      * econs 2; eauto.
-      * ss. eapply TViewFacts.write_fence_tview_mon; eauto.
-        { eapply TViewFacts.read_fence_tview_mon; eauto. refl. }
-        { refl. }
-        { eapply tview_read_fence_wf; eauto. }
-      * ss. eapply TViewFacts.write_fence_sc_mon; eauto.
-        { eapply TViewFacts.read_fence_tview_mon; eauto. refl. }
-        { refl. }
-    + inv LOCAL0. ss. clarify. esplits; eauto.
-      * econs 2; eauto.
-      * ss. eapply TViewFacts.write_fence_tview_mon; eauto.
-        { eapply TViewFacts.read_fence_tview_mon; eauto. }
-        { eapply tview_read_fence_wf; eauto. }
-      * ss. eapply TViewFacts.write_fence_sc_mon; eauto.
-        { eapply TViewFacts.read_fence_tview_mon; eauto. }
-    + inv LOCAL0. ss. clarify. esplits; eauto.
-      * econs 2; eauto. econs; eauto. econs; eauto.
-        econs; eauto. eapply promise_consistent_mon; eauto.
-Qed.
-
-Lemma progressable_in_added_rtc
-      lang st lc sc0 sc1 m0 m1 tm
-      (CONSISTENT: Thread.consistent (Thread.mk lang st lc sc0 m0))
-      (FUTURE: Memory.future m0 m1)
-  :
-    exists m2 e2,
-      (<<ADDED: rtc (added_memory tm) m1 m2>>) /\
-      (<<STEPS: rtc (Thread.tau_step (lang:=lang))
-                    (Thread.mk _ st lc sc1 m1) e2>>) /\
-      (<<PROMISES: Local.promises (Thread.local e2) = Memory.bot>>).
-Proof.
-Admitted.
-
-Definition same_locs_memory (L: Loc.t -> Prop) (mem_src mem_tgt: Memory.t): Prop :=
-  forall loc (SAT: L loc) to,
-    Memory.get loc to mem_src = Memory.get loc to mem_tgt.
-
-Definition locs_in (L: Loc.t -> Prop) (e : ThreadEvent.t) : Prop :=
-  match e with
-  | ThreadEvent.promise loc _ _ _ _ => L loc
-  | ThreadEvent.read loc _ _ _ _ => L loc
-  | ThreadEvent.write loc _ _ _ _ _ => L loc
-  | ThreadEvent.update loc _ _ _ _ _ _ _ _=> L loc
-  | _ => True
-  end.
-
-Lemma same_locs_memory_remove L mem_src0 mem_tgt0
-      loc from to msg mem_tgt1
-      (SAMELOCS: same_locs_memory L mem_src0 mem_tgt0)
-      (REMOVE: Memory.remove mem_tgt0 loc from to msg mem_tgt1)
-      (SAT: L loc)
-  :
-    exists mem_src1,
-      (<<REMOVE: Memory.remove mem_src0 loc from to msg mem_src1>>) /\
-      (<<SAMELOCS: same_locs_memory L mem_src1 mem_tgt1>>).
-Proof.
-  exploit Memory.remove_get0; eauto. i. des.
-  exploit Memory.remove_exists.
-  - erewrite SAMELOCS; eauto.
-  - i. des. esplits; eauto.
-    ii. erewrite (@Memory.remove_o mem2); eauto.
-    erewrite (@Memory.remove_o mem_tgt1); cycle 1; eauto.
-    des_ifs. eapply SAMELOCS; eauto.
-Qed.
-
-Lemma same_locs_memory_promise L mem_src0 mem_tgt0 prom0
-      loc from to msg prom1 mem_tgt1 kind
-      (SAMELOCS: same_locs_memory L mem_src0 mem_tgt0)
-      (PROMISE: Memory.promise prom0 mem_tgt0 loc from to msg prom1 mem_tgt1 kind)
-      (SAT: L loc)
-  :
-    exists mem_src1,
-      (<<PROMISE: Memory.promise prom0 mem_src0 loc from to msg prom1 mem_src1 kind>>) /\
-      (<<SAMELOCS: same_locs_memory L mem_src1 mem_tgt1>>).
-Proof.
-  inv PROMISE.
-  - dup MEM. inv MEM0. inv ADD.
-    exploit Memory.add_exists.
-    + instantiate (1:=to). instantiate (1:=from).
-      instantiate (1:=mem_src0). instantiate (1:=loc).
-      ii. exploit SAMELOCS; eauto.
-      unfold Memory.get, Cell.get. i.
-      eapply DISJOINT; eauto. erewrite <- x0. eauto.
-    + eauto.
-    + eauto.
-    + i. des. exists mem2. esplits; eauto.
-      * econs 1; eauto. i.
-Admitted.
-
-Lemma same_locs_memory_write L mem_src0 mem_tgt0 prom0
-      loc from to val vw prom1 mem_tgt1 kind
-      (SAMELOCS: same_locs_memory L mem_src0 mem_tgt0)
-      (PROMISE: Memory.write prom0 mem_tgt0 loc from to val vw prom1 mem_tgt1 kind)
-      (SAT: L loc)
-  :
-    exists mem_src1,
-      (<<PROMISE: Memory.write prom0 mem_src0 loc from to val vw prom1 mem_src1 kind>>) /\
-      (<<SAMELOCS: same_locs_memory L mem_src1 mem_tgt1>>).
-Proof.
-  inv PROMISE. exploit same_locs_memory_promise; eauto. i. des.
-  esplits; eauto.
-Qed.
-
-Lemma same_locs_memory_step
-      L lang prom th_src th_tgt th_tgt' st st' v v' prom' sc sc'
-      mem_src mem_tgt mem_tgt' tf e
-      (TH_SRC: th_src = Thread.mk lang st (Local.mk v prom) sc mem_src)
-      (TH_TGT0: th_tgt = Thread.mk lang st (Local.mk v prom) sc mem_tgt)
-      (TH_TGT1: th_tgt' = Thread.mk lang st' (Local.mk v' prom') sc' mem_tgt')
-      (SAMELOCS: same_locs_memory L mem_src mem_tgt)
-      (STEP: pred_step (locs_in L) e th_tgt th_tgt')
-  :
-    exists mem_src',
-      (<<STEP: Thread.step
-                 tf e th_src
-                 (Thread.mk lang st' (Local.mk v' prom') sc' mem_src')>>) /\
-      (<<SAMELOCS: same_locs_memory L mem_src' mem_tgt' >>)
-.
-Proof.
-  clarify. inv STEP. inv STEP0. inv STEP.
-  - inv STEP0. inv LOCAL. ss. clarify.
-    exploit same_locs_memory_promise; eauto. i. des.
-    exists mem_src1. esplits; eauto.
-    econs 1; eauto. econs; eauto.
-    + econs; eauto. eauto.
-Admitted.
